theories/examples/rand.v
@@ -23,8 +23,8 @@ Section proof.
     pose (Φ1 := (λ v, ∃ (l : loc), ⌜v = #l⌝ ∗ l ↦ₗ #true)%I).
     pose (Φ2 := (λ v, ∃ (l : loc), ⌜v = #l⌝ ∗ l ↦ᵣ #true)%I).
     iApply (dwp_atomic_lift_wp Φ1 Φ2).
-    { rewrite /WP1 /Φ1. wp_alloc l1 as "Hl". eauto with iFrame. }
-    { rewrite /WP2 /Φ2. wp_alloc l1 as "Hl". eauto with iFrame. }
+    { rewrite /TWP1 /Φ1. wp_alloc l1 as "Hl". eauto with iFrame. }
+    { rewrite /TWP2 /Φ2. wp_alloc l1 as "Hl". eauto with iFrame. }
     iIntros (? ?).
     iDestruct 1 as (l1 ->) "Hl1".
     iDestruct 1 as (l2 ->) "Hl2". clear Φ1 Φ2.
@@ -41,17 +41,17 @@ Section proof.
       pose (Φ1 := (λ v, ⌜v = #()⌝ ∗ l1 ↦ₗ #false)%I).
       pose (Φ2 := (λ v, ⌜v = #()⌝ ∗ l2 ↦ᵣ #false)%I).
       iApply dwp_atomic.
-      iInv N as (b) "[Hl1 Hl2]" "Hcl". iModIntro.
+      iInv N as (b) "[>Hl1 >Hl2]" "Hcl". iModIntro.
       iApply (dwp_atomic_lift_wp Φ1 Φ2 with "[Hl1] [Hl2] [-]"); try done.
-      - rewrite /WP1 /Φ1. wp_store. eauto.
-      - rewrite /WP2 /Φ2. wp_store. eauto.
+      - rewrite /TWP1 /Φ1. wp_store. eauto.
+      - rewrite /TWP2 /Φ2. wp_store. eauto.
       - iIntros (? ?) "[-> Hl1] [-> Hl2]". iNext.
         iMod ("Hcl" with "[-]") as "_".
         + iNext. iExists false. iFrame.
         + iModIntro. eauto. }
     iIntros (? ?) "[-> ->]". dwp_pures=>/=.
     iApply dwp_atomic; try done.
-    iInv N as (b) "[Hl1 Hl2]" "Hcl".
+    iInv N as (b) "[>Hl1 >Hl2]" "Hcl".
     iModIntro. iApply (dwp_load with "Hl1 Hl2").
     iIntros "Hl1 Hl2". iNext.
     iMod ("Hcl" with "[-]") as "_".
